\appendix
\addappheadtotoc
%\chapter{Appendices}
\setcounter{table}{0}
\renewcommand{\thetable}{A\arabic{table}}

\setcounter{figure}{0}
\renewcommand{\thefigure}{B\arabic{figure}}

\section{Partial derivative of the inverse quadratic form} \label{app1}

In this section, it will be shown that the $i^{th}$ partial derivative of:
\begin{align}
  f(\bm{x}) & = \bm{v}^T (\bm{A}(\bm{x}))^{-1} \bm{v}
\end{align}
is
\begin{align}
  \frac{\partial f}{\partial x_i} & = -\bm{y}^T \frac{\partial \bm{A}}{\partial x_i} \bm{y}^T
\end{align}
where $\bm{A}$ is a matrix-valued function of $\bm{x}$, $\bm{v}$ is a constant vector and $\bm{y} = \bm{A}^{-1} \bm{v}$ is a an implicit function of $\bm{x}$ because $\bm{A}$ is a function of $\bm{x}$.

\begin{align}
  \bm{v} & = \bm{A} \bm{y} \\
  \bm{0} & = \bm{A} \frac{\partial \bm{y}}{\partial x_i} + \frac{\partial \bm{A}}{\partial x_i} \bm{y} \\
  \frac{\partial y}{\partial x_i} & = - \bm{A}^{-1} \frac{\partial \bm{A}}{\partial x_i} \bm{y} \\
  f(\bm{x}) & = \bm{v}^T \bm{A}^{-1} \bm{v} \\
  & = \bm{y}^T \bm{A} \bm{y} \\
  \frac{\partial f}{\partial x_i} & = 2 \bm{y}^T \bm{A} \frac{\partial \bm{y}}{\partial x_i} + \bm{y}^T \frac{\partial \bm{A}}{\partial x_i} \bm{y} \\
  & = - 2 \bm{y}^T \bm{A} \bm{A}^{-1} \frac{\partial \bm{A}}{\partial x_i} \bm{y} + \bm{y}^T \frac{\partial \bm{A}}{\partial x_i} \bm{y} \\
  & = - 2 \bm{y}^T \frac{\partial \bm{A}}{\partial x_i} \bm{y} + \bm{y}^T \frac{\partial \bm{A}}{\partial x_i} \bm{y} \\
  & = - \bm{y}^T \frac{\partial \bm{A}}{\partial x_i} \bm{y}
\end{align}
